src/extraction.v
@@ -7,11 +7,16 @@ From array Require Import wp.
 Extraction Inline bind.
 
 From Stdlib Require ExtrOCamlInt63.
+
+From array Require Import iteration.
+Extraction Inline did_break did_not_break.
+
 From array Require Import int.
+Extraction Inline down iter_up xiter_up uxiter_up.
 
 (* Recursive Extraction down up interruptible_up interruptible_up_unit. *)
 
 From Stdlib Require ExtrOCamlPArray.
-From array Require Import array specialization.
+From array Require Import array.
 
 (* Recursive Extraction of_list blit blit' copy find_index equal. *)
